CtLean/CCS.lean
@@ -1,0 +1,55 @@
+import CtLean.Basic
+
+inductive Act (names: Type) where
+| name (_: names)
+| coname (_: names)
+| tau
+
+inductive CCS (N: Type) (K: Type): Type
+| nil
+| pref (act: Act N) (p: CCS N K)
+| par (left: CCS N K) (right: CCS N K)
+| choice (left: CCS N K) (right: CCS N K)
+| abst (var: N) (p: CCS N K)
+| const (k: K)
+
+class Konst (N: Type) (K: Type) where
+  acts (k: K): Act N -> Prop
+  resolve (k: K): (a: Act N) → acts k a → CCS N K
+
+inductive Complementary: Act N → Act N → Prop
+| left: Complementary (.name n) (.coname n)
+| right: Complementary (.coname n) (.name n)
+
+inductive Transition [kdef: Konst N K]: CCS N K -> Act N -> CCS N K -> Prop
+| Pre: Transition (.pref a p) a p
+| ParL (h: Transition p a p'): Transition (.par p q) a (.par p' q)
+| ParR (h: Transition q a q'): Transition (.par p q) a (.par p q')
+| Com
+  (l: Transition p a p')
+  (r: Transition q a' q')
+  (_: Complementary a a'):
+  Transition (.par p q) .tau (.par p' q')
+| SumL (h: Transition p a p'): Transition (.choice p q) a p'
+| SumR (h: Transition q a q'): Transition (.choice p q) a q'
+| Res
+  (h: Transition p a p')
+  (not_name: a ≠ .name n)
+  (not_coname: a ≠ .coname n):
+  Transition (.abst n p) a (.abst n q)
+| Rec
+  (h: kdef.acts k a)
+  (r: p = kdef.resolve k a h):
+  Transition (.const k) a p
+
+instance [Konst N K] : LTS (CCS N K) where
+  Act := Act N
+  transition := @Transition N K _
+
+variable [Konst N K] (p q: CCS N K)
+
+theorem bisim_choice: Bisimilar p q → Bisimilar p (CCS.choice p q) := by
+  intros
+  constructor
+  sorry
+  sorry
