CtLean/Coind.lean
@@ -1,0 +1,122 @@
+import «CtLean».Basic
+
+variable [LTS P] (p q: P)
+
+
+structure LTS.Edge (p: P) where
+  act: LTS.Act P
+  dest: P
+  prop: transition p act dest
+
+inductive LTS.Path: P → Type
+| nil (p: P): Path p
+| cons {p p': P} (ps: Path p) (e: Edge p) (h: e.dest = p'): Path p'
+
+def LTS.Path.orig: ∀{p: P}, (LTS.Path p) → P
+| p, nil _ => p
+| _, cons ps _ _ => ps.orig
+
+
+def Simulate (p q: P) (map: ∀(p: P), LTS.Edge p → P → P): Nat → Prop
+| 0 => True
+| .succ n => ∀(e: LTS.Edge p),
+  (LTS.transition q e.act (map p e q) ∧ Simulate e.dest (map p e q) map n)
+
+structure Bisimulation' where
+  sim: ∀(p: P), LTS.Edge p → P → P
+  sym: ∀{a}, ∀{p p' q}, ∀t, ∀t', sim q ⟨a, sim p ⟨a, p', t⟩ q, t'⟩ p = p'
+  coind_l: ∀n, Simulate p q sim n
+  coind_r: ∀n, Simulate q p sim n
+
+def Bisimilar' := Nonempty (Bisimulation' p q)
+
+def SelfSim: Bisimulation' p p where
+  sim p e _ := e.dest
+  sym _ _ := rfl
+  coind_l n := by
+    induction n generalizing p with
+    | zero => trivial
+    | succ n ih => refine fun ⟨_, _, prop⟩ => ⟨prop, ih _⟩
+  coind_r n := by
+    induction n generalizing p with
+    | zero => trivial
+    | succ n ih => refine fun ⟨_, _, prop⟩ => ⟨prop, ih _⟩
+
+theorem Bisimilar'.refl: Bisimilar' p p :=
+  ⟨SelfSim p⟩
+
+def InvSim (h: Bisimulation' p q): Bisimulation' q p where
+  sim := h.sim
+  sym := h.sym
+  coind_l := h.coind_r
+  coind_r := h.coind_l
+
+theorem Bisimilar'.symm: Bisimilar' p q → Bisimilar' q p :=
+  fun ⟨h⟩ => ⟨InvSim _ _ h⟩
+
+structure BisimCond: Prop where
+  left: LTS.transition p a p' → ∃q', (LTS.transition q a q' ∧ Bisimilar p' q')
+  right: LTS.transition q a q' → ∃p', (LTS.transition p a p' ∧ Bisimilar p' q')
+
+theorem BisimCond.refl: BisimCond p p where
+  left t := ⟨_, ⟨t, Bisimilar.refl _⟩⟩
+  right t := ⟨_, ⟨t, Bisimilar.refl _⟩⟩
+
+theorem BisimCond.symm (h: BisimCond p q): BisimCond q p where
+  left t := by
+    have ⟨_, ⟨t', h'⟩⟩ := h.right t
+    refine ⟨_, ⟨t', h'.symm⟩⟩
+
+  right t := by
+    have ⟨_, ⟨t', h'⟩⟩ := h.left t
+    refine ⟨_, ⟨t', h'.symm⟩⟩
+
+theorem show_cond: Bisimilar' p q → BisimCond p q := by
+  intro ⟨sim, sym, coind_l, coind_r⟩
+  constructor
+  . intro _ _ t
+    let e: LTS.Edge _ := ⟨_, _, t⟩
+    exists (sim p e q)
+    constructor
+    . exact (coind_l 1 e).left
+    . refine ⟨sim, sym, ?_, ?_⟩
+      . intro n
+        refine (coind_l n.succ e).right
+      . intro n
+        let e': LTS.Edge _ := ⟨_, _, (coind_l n.succ e).left⟩
+        have := sym e.prop e'.prop ▸ (coind_r n.succ e').right
+        exact this
+  . intro _ _ t
+    let e: LTS.Edge _ := ⟨_, _, t⟩
+    exists (sim q e p)
+    constructor
+    . exact (coind_r 1 e).left
+    . refine ⟨sim, sym, ?_, ?_⟩
+      . intro n
+        let e': LTS.Edge _ := ⟨_, _, (coind_r n.succ e).left⟩
+        have := sym e.prop e'.prop ▸ (coind_l n.succ e').right
+        exact this
+      . intro n
+        refine (coind_r n.succ e).right
+
+noncomputable def sim [DecidableEq P] {p q: P} (h: BisimCond p q):
+  ∀(p': P), LTS.Edge p' → P → P := fun p ⟨a, p', t⟩ q =>
+    sorry
+
+theorem sim_edge [DecidableEq P]: (t: LTS.transition p a p') →
+  LTS.transition q a (sim h _ ⟨_, _, t⟩ q) :=
+  sorry
+
+theorem sim_cond [DecidableEq P] (h: BisimCond p q)
+  (lp: {ps: LTS.Path p' // ps.orig = p})
+  (rp: {qs: LTS.Path q' // qs.orig = q}):
+  ∀n, Simulate p' q' (sim h) n := by
+  intro n; cases n; trivial
+  case succ n' =>
+    intro e
+    constructor
+    . apply sim_edge
+    . apply sim_cond
+      . refine ⟨LTS.Path.cons lp.val e rfl, lp.property⟩
+      . let e' : LTS.Edge _ := ⟨_, _, sim_edge (h:=h) p' q' e.prop⟩
+        refine ⟨LTS.Path.cons rp.val e' rfl, rp.property⟩
